adding a memory and invariants layer on top of pcm heaps

ulib/experimental/Steel.PCM.Heap.fsti
@@ -13,26 +13,28 @@
    See the License for the specific language governing permissions and
    limitations under the License.
 *)
-module Steel.PCM.Memory
+module Steel.PCM.Heap
 open FStar.Ghost
 open Steel.PCM
 
-/// Abstract type of memories
-val mem  : Type u#(a + 1)
-val core_mem (m:mem u#a) : mem u#a
+/// Abstract type of heaps
+val heap  : Type u#(a + 1)
 
-/// A predicate describing non-overlapping memories
-val disjoint (m0 m1:mem u#h) : prop
+/// A heap maps a reference to its associated value
+val ref (a:Type u#a) (pcm:pcm a) : Type u#0
+
+/// A predicate describing non-overlapping heaps
+val disjoint (m0 m1:heap u#h) : prop
 
 /// disjointness is symmetric
-val disjoint_sym (m0 m1:mem u#h)
+val disjoint_sym (m0 m1:heap u#h)
   : Lemma (disjoint m0 m1 <==> disjoint m1 m0)
           [SMTPat (disjoint m0 m1)]
 
-/// disjoint memories can be combined
-val join (m0:mem u#h) (m1:mem u#h{disjoint m0 m1}) : mem u#h
+/// disjoint heaps can be combined
+val join (m0:heap u#h) (m1:heap u#h{disjoint m0 m1}) : heap u#h
 
-val join_commutative (m0 m1:mem)
+val join_commutative (m0 m1:heap)
   : Lemma
     (requires
       disjoint m0 m1)
@@ -41,7 +43,7 @@ val join_commutative (m0 m1:mem)
        join m0 m1 == join m1 m0))
 
 /// disjointness distributes over join
-val disjoint_join (m0 m1 m2:mem)
+val disjoint_join (m0 m1 m2:heap)
   : Lemma (disjoint m1 m2 /\
            disjoint m0 (join m1 m2) ==>
            disjoint m0 m1 /\
@@ -49,7 +51,7 @@ val disjoint_join (m0 m1 m2:mem)
            disjoint (join m0 m1) m2 /\
            disjoint (join m0 m2) m1)
 
-val join_associative (m0 m1 m2:mem)
+val join_associative (m0 m1 m2:heap)
   : Lemma
     (requires
       disjoint m1 m2 /\
@@ -58,23 +60,25 @@ val join_associative (m0 m1 m2:mem)
       (disjoint_join m0 m1 m2;
        join m0 (join m1 m2) == join (join m0 m1) m2))
 
-/// The type of mem assertions
-//[@@erasable] I would like this to be abstract, but I can't define an abstract abbreviation of an erasable type and have it be erasable too. Need to fix that
-let slprop = Steel.PCM.Heap.slprop
+let heap_prop_is_affine (p:heap u#a -> prop) : prop =
+  forall (h0 h1: heap u#a). p h0 /\ disjoint h0 h1 ==> p (join h0 h1)
 
-/// interpreting mem assertions as memory predicates
-val interp (p:slprop u#a) (m:mem u#a) : prop
+let a_heap_prop : Type u#(a + 1) = p:(heap u#a -> prop) { heap_prop_is_affine p }
 
-/// A common abbreviation: memories validating p
-let hmem (p:slprop u#a) = m:mem u#a {interp p m}
+/// The type of heap assertions
+[@@erasable]
+val slprop : Type u#(a + 1)
+
+/// interpreting heap assertions as heapory predicates
+val interp (p:slprop u#a) (m:heap u#a) : prop
+
+/// A common abbreviation: heaps validating p
+let hheap (p:slprop u#a) = m:heap u#a {interp p m}
 
 /// Equivalence relation on slprops is just
 /// equivalence of their interpretations
 let equiv (p1 p2:slprop) =
   forall m. interp p1 m <==> interp p2 m
-
-/// A heap maps a reference to its associated value
-val ref (a:Type u#a) (pcm:pcm a) : Type u#0
 
 /// All the standard connectives of separation logic
 val emp : slprop u#a
@@ -85,6 +89,7 @@ val star  (p1 p2:slprop u#a) : slprop u#a
 val wand  (p1 p2:slprop u#a) : slprop u#a
 val h_exists (#a:Type u#a) (f: (a -> slprop u#a)) : slprop u#a
 val h_forall (#a:Type u#a) (f: (a -> slprop u#a)) : slprop u#a
+val h_refine (p:slprop u#a) (r:a_heap_prop u#a) : slprop u#a
 
 ////////////////////////////////////////////////////////////////////////////////
 //properties of equiv
@@ -96,10 +101,13 @@ val equiv_symmetric (p1 p2:slprop)
 val equiv_extensional_on_star (p1 p2 p3:slprop)
   : squash (p1 `equiv` p2 ==> (p1 `star` p3) `equiv` (p2 `star` p3))
 
+(** Properties of emp *)
+val emp_unit (p:slprop)
+  : Lemma (p `equiv` (p `star` emp))
 
 ////////////////////////////////////////////////////////////////////////////////
 // pts_to and abbreviations
-////////////////////////////////////////////////////////////////////////////////
+//////////////////////////////////////////////////////////////////////////////////////////
 let ptr #a #pcm (r:ref a pcm) =
     h_exists (pts_to r)
 
@@ -107,7 +115,7 @@ val pts_to_compatible (#a:Type u#a)
                       (#pcm:_)
                       (x:ref a pcm)
                       (v0 v1:a)
-                      (m:mem u#a)
+                      (m:heap u#a)
   : Lemma
     (requires
       interp (pts_to x v0 `star` pts_to x v1) m)
@@ -119,7 +127,7 @@ val pts_to_compatible (#a:Type u#a)
 // star
 ////////////////////////////////////////////////////////////////////////////////
 
-val intro_star (p q:slprop) (mp:hmem p) (mq:hmem q)
+val intro_star (p q:slprop) (mp:hheap p) (mq:hheap q)
   : Lemma
     (requires
       disjoint mp mq)
@@ -138,84 +146,92 @@ val star_congruence (p1 p2 p3 p4:slprop)
   : Lemma (requires p1 `equiv` p3 /\ p2 `equiv` p4)
           (ensures (p1 `star` p2) `equiv` (p3 `star` p4))
 
-val affine_star (p q:slprop) (m:mem)
+val affine_star (p q:slprop) (m:heap)
   : Lemma ((interp (p `star` q) m ==> interp p m /\ interp q m))
 
 ////////////////////////////////////////////////////////////////////////////////
-// Memory invariants
+// refine
 ////////////////////////////////////////////////////////////////////////////////
-val lock_addr : eqtype
-module S = FStar.Set
 
-val locks_invariant (e:S.set lock_addr) (m:mem u#a) : slprop u#a
+val refine_interp (p:slprop u#a) (q:a_heap_prop u#a) (h:heap u#a)
+    : Lemma (interp p h /\ q h <==> interp (h_refine p q) h)
 
-let hmem_with_inv' (e:S.set lock_addr) (fp:slprop u#a) =
-  m:mem{interp (fp `star` locks_invariant e m) m}
+val refine_equiv (p0 p1:slprop u#a) (q0 q1:a_heap_prop u#a)
+    : Lemma (p0 `equiv` p1 /\ (forall h. q0 h <==> q1 h) <==>
+             equiv (h_refine p0 q0) (h_refine p1 q1))
 
-let hmem_with_inv (fp:slprop u#a) =
-  m:mem u#a{interp (fp `star` locks_invariant Set.empty m) m}
+////////////////////////////////////////////////////////////////////////////////
+// Actions:
+////////////////////////////////////////////////////////////////////////////////
+val free_above_addr (h:heap u#a) (a:nat) : prop
+
+(** A heap predicate that depends only on fp *)
+let hprop (fp:slprop u#a) =
+  q:(heap u#a -> prop){
+    forall (m0:heap{interp fp m0}) (m1:heap{disjoint m0 m1}).
+      q m0 <==> q (join m0 m1)}
+
+let pre_action (fp:slprop) (a:Type) (fp':a -> slprop) =
+  hheap fp -> (x:a & hheap (fp' x))
+
+let is_frame_preserving #a #fp #fp' (f:pre_action fp a fp') =
+   forall frame (h0:hheap (fp `star` frame)).
+     (affine_star fp frame h0;
+      let (| x, h1 |) = f h0 in
+      interp (fp' x `star` frame) h1 /\
+      (forall ctr. h0 `free_above_addr` ctr <==> h1 `free_above_addr` ctr) /\
+      (forall (hp:hprop frame). hp h0 == hp h1))
 
 
-(***** Following lemmas are needed in Steel.Effect *****)
+let action (fp:slprop) (a:Type) (fp':a -> slprop) =
+  f:pre_action fp a fp'{ is_frame_preserving f }
 
-val core_mem_interp (hp:slprop u#a) (m:mem u#a)
-    : Lemma
-      (requires interp hp m)
-      (ensures interp hp (core_mem m))
-      [SMTPat (interp hp (core_mem m))]
+let frame_related_heaps (h0 h1:heap) (fp0 fp1 frame:slprop) =
+  interp (fp0 `star` frame) h0 /\
+  interp (fp1 `star` frame) h1 /\
+  (forall ctr. h0 `free_above_addr` ctr <==> h1 `free_above_addr` ctr) /\
+  (forall (hp:hprop frame). hp h0 == hp h1)
+
+let action_framing #a #fp #fp' ($f:action fp a fp')
+                         (frame:slprop) (h0:hheap (fp `star` frame))
+  : Lemma (affine_star fp frame h0;
+           let (| x, h1 |) = f h0 in
+           frame_related_heaps h0 h1 fp (fp' x) frame)
+  = affine_star fp frame h0;
+    emp_unit fp
+
+(** Reading *)
+val sel (#a:_) (#pcm:_) (r:ref a pcm) (m:hheap (ptr r))
+  : a
+
+/// sel respect pts_to
+val sel_lemma (#a:_) (#pcm:_) (r:ref a pcm) (m:hheap (ptr r))
+  : Lemma (interp (pts_to r (sel r m)) m)
+
+val sel_action (#a:_) (#pcm:_) (r:ref a pcm) (v0:erased a)
+  : action (pts_to r v0) (v:a{compatible pcm v0 v}) (fun _ -> pts_to r v0)
+
+(** Writing *)
+/// updating a ref cell from v0 to v1
+/// must be compatible with other views of the same cell
+val upd_action (#a:_) (#pcm:_) (r:ref a pcm)
+               (v0:FStar.Ghost.erased a)
+               (v1:a {Steel.PCM.frame_preserving pcm v0 v1})
+  : action (pts_to r v0) unit (fun _ -> pts_to r v1)
+
+(** Allocating, pseudo action *)
+val extend (#a:_) (#pcm:_) (x:a) (addr:nat)
+           (h:heap{h `free_above_addr` addr})
+  : (r:ref a pcm & h':heap{(forall f. interp f h ==> interp f h') /\
+                           interp (pts_to r x) h' /\
+                           h' `free_above_addr` (addr + 1)})
 
 val interp_depends_only_on (hp:slprop u#a)
     : Lemma
-      (forall (m0:hmem hp) (m1:mem u#a{disjoint m0 m1}).
+      (forall (m0:hheap hp) (m1:heap u#a{disjoint m0 m1}).
         interp hp m0 <==> interp hp (join m0 m1))
-
-let affine_star_smt (p q:slprop u#a) (m:mem u#a)
-    : Lemma (interp (p `star` q) m ==> interp p m /\ interp q m)
-      [SMTPat (interp (p `star` q) m)]
-    = affine_star p q m
 
 val h_exists_cong (#a:Type) (p q : a -> slprop)
     : Lemma
       (requires (forall x. p x `equiv` q x))
       (ensures (h_exists p `equiv` h_exists q))
-
-////////////////////////////////////////////////////////////////////////////////
-// Actions:
-////////////////////////////////////////////////////////////////////////////////
-
-(** A memory predicate that depends only on fp *)
-let mprop (fp:slprop u#a) =
-  q:(mem u#a -> prop){
-    forall (m0:mem{interp fp m0}) (m1:mem{disjoint m0 m1}).
-      q m0 <==> q (join m0 m1)}
-
-let pre_action (fp:slprop u#a) (a:Type u#b) (fp':a -> slprop u#a) =
-  hmem_with_inv fp -> (x:a & hmem_with_inv (fp' x))
-
-val ac_reasoning_for_m_frame_preserving
-    (p q r:slprop u#a) (m:mem u#a)
-  : Lemma
-    (requires interp ((p `star` q) `star` r) m)
-    (ensures interp (p `star` r) m)
-
-let is_frame_preserving
-  (#a:Type u#b)
-  (#fp:slprop u#a)
-  (#fp':a -> slprop u#a)
-  (f:pre_action u#a u#b fp a fp') =
-  forall (frame:slprop u#a) (m0:hmem_with_inv (fp `star` frame)).
-    (ac_reasoning_for_m_frame_preserving fp frame (locks_invariant Set.empty m0) m0;
-     let (| x, m1 |) = f m0 in
-     interp ((fp' x `star` frame) `star` locks_invariant Set.empty m1) m1 /\
-     (forall (mp:mprop frame). mp (core_mem m0) == mp (core_mem m1)))
-
-let action (fp:slprop u#a) (a:Type u#b) (fp':a -> slprop u#a) =
-  f:pre_action fp a fp'{ is_frame_preserving f }
-
-val sel_action (#a:_) (#pcm:_) (r:ref a pcm) (v0:erased a)
-  : action (pts_to r v0) (v:a{compatible pcm v0 v}) (fun _ -> pts_to r v0)
-
-val upd_action (#a:_) (#pcm:_) (r:ref a pcm)
-               (v0:FStar.Ghost.erased a)
-               (v1:a {Steel.PCM.frame_preserving pcm v0 v1})
-  : action (pts_to r v0) unit (fun _ -> pts_to r v1)
