ulib/experimental/Steel.PCM.Memory.fst
@@ -17,639 +17,294 @@ module Steel.PCM.Memory
 module F = FStar.FunctionalExtensionality
 open FStar.FunctionalExtensionality
 open Steel.PCM
+module H = Steel.PCM.Heap
 
-// In the future, we may have other cases of cells
-// for arrays and structs
 noeq
-type cell : Type u#(a + 1) =
-  | Ref : a:Type u#a ->
-          p:pcm a ->
-          v:a ->
-          cell
+type lock_state : Type u#(a + 1) =
+  | Invariant : H.slprop u#a -> lock_state
 
-let addr = nat
+let lock_store : Type u#(a+1) = list (lock_state u#a)
 
-/// This is just the core of a memory, about which one can write
-/// assertions. At one level above, we'll encapsulate this memory
-/// with a freshness counter, a lock store etc.
-let heap : Type u#(a + 1) = addr ^-> option (cell u#a)
-
-let contains_addr (m:heap) (a:addr)
-  : bool
-  = Some? (m a)
-
-let select_addr (m:heap) (a:addr{contains_addr m a})
-  : cell
-  = Some?.v (m a)
-
-let update_addr (m:heap) (a:addr) (c:cell)
-  : heap
-  = F.on _ (fun a' -> if a = a' then Some c else m a')
-
-let disjoint_cells (c0 c1:cell u#h) : prop =
-    let Ref t0 p0 v0 = c0 in
-    let Ref t1 p1 v1 = c1 in
-    t0 == t1 /\
-    p0 == p1 /\
-    composable p0 v0 v1
-
-let disjoint_cells_sym (c0 c1:cell u#h)
-  : Lemma (requires disjoint_cells c0 c1)
-          (ensures disjoint_cells c1 c0)
-  = let Ref t0 p0 v0 = c0 in
-    let Ref t1 p1 v1 = c1 in ()
-
-let disjoint_addr (m0 m1:heap u#h) (a:addr)
-  : prop
-  = match m0 a, m1 a with
-    | Some c0, Some c1 ->
-      disjoint_cells c0 c1
-    | Some _, None
-    | None, Some _
-    | None, None ->
-      True
-
-let ref (a:Type u#a) (pcm:pcm a): Type u#0 = addr
-
-let disjoint (m0 m1:heap u#h)
-  : prop
-  = forall a. disjoint_addr m0 m1 a
-
-#push-options "--warn_error -271"
-
-let disjoint_sym (m0 m1:heap u#h)
-  = let aux (m0 m1:heap u#h) (a:addr)
-      : Lemma (requires disjoint_addr m0 m1 a)
-              (ensures disjoint_addr m1 m0 a)
-              [SMTPat (disjoint_addr m1 m0 a)]
-    = match m0 a, m1 a with
-      | Some c0, Some c1 -> disjoint_cells_sym c0 c1
-      | _ -> ()
-    in
-    ()
-
-let join_cells (c0:cell u#h) (c1:cell u#h{disjoint_cells c0 c1}) =
-  let Ref a0 p0 v0 = c0 in
-  let Ref a1 p1 v1 = c1 in
-  Ref a0 p0 (op p0 v0 v1)
-
-let join (m0:heap) (m1:heap{disjoint m0 m1})
-  : heap
-  = F.on _ (fun a ->
-      match m0 a, m1 a with
-      | None, None -> None
-      | None, Some x -> Some x
-      | Some x, None -> Some x
-      | Some c0, Some c1 ->
-        Some (join_cells c0 c1))
-
-let disjoint_join_cells_assoc (c0 c1 c2:cell u#h)
-  : Lemma
-    (requires disjoint_cells c1 c2 /\
-              disjoint_cells c0 (join_cells c1 c2))
-    (ensures  disjoint_cells c0 c1 /\
-              disjoint_cells (join_cells c0 c1) c2 /\
-              join_cells (join_cells c0 c1) c2 == join_cells c0 (join_cells c1 c2))
-  = let Ref a0 p0 v0 = c0 in
-    let Ref a1 p1 v1 = c1 in
-    let Ref a2 p2 v2 = c2 in
-    p0.assoc v0 v1 v2
-
-let disjoint_join' (m0 m1 m2:heap u#h)
-  : Lemma (requires disjoint m1 m2 /\
-                    disjoint m0 (join m1 m2))
-          (ensures  disjoint m0 m1 /\ disjoint (join m0 m1) m2)
-          [SMTPat (disjoint (join m0 m1) m2)]
-  = let aux (a:addr)
-      : Lemma (disjoint_addr m0 m1 a)
-              [SMTPat ()]
-      = match m0 a, m1 a, m2 a with
-        | Some c0, Some c1, Some c2 ->
-          disjoint_join_cells_assoc c0 c1 c2
-        | _ -> ()
-    in
-    assert (disjoint m0 m1);
-    let aux (a:addr)
-      : Lemma (disjoint_addr (join m0 m1) m2 a)
-              [SMTPat ()]
-      = match m0 a, m1 a, m2 a with
-        | Some c0, Some c1, Some c2 ->
-          disjoint_join_cells_assoc c0 c1 c2
-        | _ -> ()
-    in
-    ()
-
-let mem_equiv (m0 m1:heap) =
-  forall a. m0 a == m1 a
-
-let mem_equiv_eq (m0 m1:heap)
-  : Lemma
-    (requires
-      m0 `mem_equiv` m1)
-    (ensures
-      m0 == m1)
-    [SMTPat (m0 `mem_equiv` m1)]
-  = F.extensionality _ _ m0 m1
-
-let join_cells_commutative (c0:cell u#h) (c1:cell u#h{disjoint_cells c0 c1})
-  : Lemma (disjoint_cells_sym c0 c1; join_cells c0 c1 == join_cells c1 c0)
-          [SMTPat (join_cells c0 c1)]
-  = let Ref a0 p0 v0 = c0 in
-    let Ref a1 p1 v1 = c1 in
-    p0.comm v0 v1
-
-let join_commutative' (m0 m1:heap)
-  : Lemma
-    (requires
-      disjoint m0 m1)
-    (ensures
-      join m0 m1 `mem_equiv` join m1 m0)
-    [SMTPat (join m0 m1)]
-  = ()
-
-let join_commutative m0 m1 = ()
-
-let disjoint_join (m0 m1 m2:heap)
-  : Lemma (disjoint m1 m2 /\
-           disjoint m0 (join m1 m2) ==>
-           disjoint m0 m1 /\
-           disjoint m0 m2 /\
-           disjoint (join m0 m1) m2 /\
-           disjoint (join m0 m2) m1)
-          [SMTPat (disjoint m0 (join m1 m2))]
-  = let aux ()
-      : Lemma
-        (requires disjoint m1 m2 /\
-                  disjoint m0 (join m1 m2))
-        (ensures  disjoint m0 m1 /\
-                  disjoint m0 m2 /\
-                  disjoint (join m0 m1) m2 /\
-                  disjoint (join m0 m2) m1)
-        [SMTPat ()]
-      = disjoint_join' m0 m1 m2;
-        join_commutative m0 m1;
-        disjoint_join' m0 m2 m1
-    in
-    ()
-
-let join_associative' (m0 m1 m2:heap)
-  : Lemma
-    (requires
-      disjoint m1 m2 /\
-      disjoint m0 (join m1 m2))
-    (ensures
-      (disjoint_join m0 m1 m2;
-       join m0 (join m1 m2) `mem_equiv` join (join m0 m1) m2))
-    [SMTPatOr
-      [[SMTPat (join m0 (join m1 m2))];
-       [SMTPat (join (join m0 m1) m2)]]]
-  = disjoint_join m0 m1 m2;
-    let l = join m0 (join m1 m2) in
-    let r = join (join m0 m1) m2 in
-    let aux (a:addr)
-        : Lemma (l a == r a)
-                [SMTPat ()]
-        = match m0 a, m1 a, m2 a with
-          | Some c0, Some c1, Some c2 ->
-            disjoint_join_cells_assoc c0 c1 c2
-          | _ -> ()
-    in
-    ()
-
-let join_associative (m0 m1 m2:heap) = join_associative' m0 m1 m2
-
-let join_associative2 (m0 m1 m2:heap)
-  : Lemma
-    (requires
-      disjoint m0 m1 /\
-      disjoint (join m0 m1) m2)
-    (ensures
-      disjoint m1 m2 /\
-      disjoint m0 (join m1 m2) /\
-      join m0 (join m1 m2) `mem_equiv` join (join m0 m1) m2)
-    [SMTPat (join (join m0 m1) m2)]
-  = disjoint_join m2 m0 m1;
-    join_commutative (join m0 m1) m2;
-    join_associative m2 m0 m1
-
-let heap_prop_is_affine (p:heap -> prop) =
-  forall m0 m1. p m0 /\ disjoint m0 m1 ==> p (join m0 m1)
-let a_heap_prop : Type u#(a + 1) =
-  p:(heap u#a -> prop) { heap_prop_is_affine p }
-
-////////////////////////////////////////////////////////////////////////////////
-
-module W = FStar.WellFounded
-
-[@@erasable]
 noeq
-type slprop : Type u#(a + 1) =
-  | Emp : slprop
-  | Pts_to : #a:Type u#a -> #pcm:pcm a -> r:ref a pcm -> v:a -> slprop
-  | Refine : slprop u#a -> a_heap_prop u#a -> slprop
-  | And    : slprop u#a -> slprop u#a -> slprop
-  | Or     : slprop u#a -> slprop u#a -> slprop
-  | Star   : slprop u#a -> slprop u#a -> slprop
-  | Wand   : slprop u#a -> slprop u#a -> slprop
-  | Ex     : #a:Type u#a -> (a -> slprop u#a) -> slprop
-  | All    : #a:Type u#a -> (a -> slprop u#a) -> slprop
+type mem : Type u#(a + 1) =
+  {
+    ctr: nat;
+    heap: H.heap u#a;
+    locks: lock_store u#a;
+  }
 
-let interp_cell (p:slprop u#a) (c:cell u#a) =
-  let Ref a' pcm' v' = c in
-  match p with
-  | Pts_to #a #pcm r v ->
-    a == a' /\
-    pcm == pcm' /\
-    compatible pcm v v'
-  | _ -> False
+let heap_of_mem (x:mem) : H.heap = x.heap
 
-let rec interp (p:slprop u#a) (m:heap u#a)
-  : Tot prop (decreases p)
-  = match p with
-    | Emp -> True
-    | Pts_to #a #pcm r v ->
-      m `contains_addr` r /\
-      interp_cell p (select_addr m r)
+let mem_of_heap (h:H.heap) : mem = {
+  ctr = 0;
+  heap = h;
+  locks = []
+}
 
-    | Refine p q ->
-      interp p m /\ q m
+let core_mem (m:mem) : mem = mem_of_heap (heap_of_mem m)
 
-    | And p1 p2 ->
-      interp p1 m /\
-      interp p2 m
+let disjoint (m0 m1:mem u#h)
+  : prop
+  = m0.ctr == m1.ctr /\
+    H.disjoint m0.heap m1.heap /\
+    m0.locks == m1.locks
 
-    | Or  p1 p2 ->
-      interp p1 m \/
-      interp p2 m
+let disjoint_sym m0 m1 = ()
 
-    | Star p1 p2 ->
-      exists m1 m2.
-        m1 `disjoint` m2 /\
-        m == join m1 m2 /\
-        interp p1 m1 /\
-        interp p2 m2
+let join m0 m1 = {
+  ctr = m0.ctr;
+  heap = H.join m0.heap m1.heap;
+  locks = m0.locks
+}
 
-    | Wand p1 p2 ->
-      forall m1.
-        m `disjoint` m1 /\
-        interp p1 m1 ==>
-        interp p2 (join m m1)
+let join_commutative m0 m1 =
+  H.join_commutative m0.heap m1.heap
 
-    | Ex f ->
-      exists x. (W.axiom1 f x; interp (f x) m)
+let disjoint_join m0 m1 m2 =
+  H.disjoint_join m0.heap m1.heap m2.heap
 
-    | All f ->
-      forall x. (W.axiom1 f x; interp (f x) m)
+let join_associative m0 m1 m2 =
+  H.join_associative m0.heap m1.heap m2.heap
 
-let emp : slprop u#a = Emp
-let pts_to = Pts_to
-let h_and = And
-let h_or = Or
-let star = Star
-let wand = Wand
-let h_exists = Ex
-let h_forall = All
+let interp p m = H.interp p m.heap
+
+let ref = H.ref
+
+let emp : slprop u#a = H.emp
+let pts_to = H.pts_to
+let h_and = H.h_and
+let h_or = H.h_or
+let star = H.star
+let wand = H.wand
+let h_exists = H.h_exists
+let h_forall = H.h_forall
 
 ////////////////////////////////////////////////////////////////////////////////
 //properties of equiv
 ////////////////////////////////////////////////////////////////////////////////
 
-let equiv_symmetric (p1 p2:slprop u#a) = ()
-let equiv_extensional_on_star (p1 p2 p3:slprop u#a) = ()
+let equiv_symmetric (p1 p2:slprop u#a) = H.equiv_symmetric p1 p2
+
+#push-options "--warn_error -271"
+let equiv_heap_iff_equiv (p1 p2:slprop u#a)
+  : Lemma (H.equiv p1 p2 <==> equiv p1 p2)
+  = let aux_lr ()
+      : Lemma
+        (requires H.equiv p1 p2)
+        (ensures equiv p1 p2)
+        [SMTPat ()]
+      = ()
+    in
+    let aux_rl_helper1 (h:H.heap)
+      : Lemma
+        (requires equiv p1 p2 /\ H.interp p1 h)
+        (ensures H.interp p2 h)
+        [SMTPat ()]
+      = assert (interp p2 (mem_of_heap h))
+    in
+    let aux_rl_helper2 (h:H.heap)
+      : Lemma
+        (requires equiv p1 p2 /\ H.interp p2 h)
+        (ensures H.interp p1 h)
+        [SMTPat ()]
+      = assert (interp p2 (mem_of_heap h))
+    in
+    let aux_rl ()
+      : Lemma
+        (requires equiv p1 p2)
+        (ensures H.equiv p1 p2)
+        [SMTPat ()]
+      = () in
+    ()
+
+let equiv_heap_iff_equiv_forall ()
+  : Lemma (ensures (forall p1 p2. H.equiv p1 p2 <==> equiv p1 p2))
+  = let aux p1 p2
+      : Lemma (ensures (H.equiv p1 p2 <==> equiv p1 p2))
+              [SMTPat ()]
+      = equiv_heap_iff_equiv p1 p2
+    in
+    ()
+#pop-options
+
+let equiv_extensional_on_star (p1 p2 p3:slprop u#a) =
+  equiv_heap_iff_equiv_forall ();
+  H.equiv_extensional_on_star p1 p2 p3
 
 ////////////////////////////////////////////////////////////////////////////////
 //pts_to
 ////////////////////////////////////////////////////////////////////////////////
 
-let intro_pts_to (#a:_) (#pcm:pcm a) (x:ref a pcm) (v:a) (m:heap)
-  : Lemma
-    (requires
-       m `contains_addr` x /\
-       (let Ref a' pcm' v' = select_addr m x in
-        a == a' /\
-        pcm == pcm' /\
-        compatible pcm v v'))
-     (ensures
-       interp (pts_to x v) m)
-  = ()
-
-
 let pts_to_compatible (#a:Type u#a)
                       (#pcm:_)
                       (x:ref a pcm)
                       (v0 v1:a)
-                      (m:heap u#a)
-  : Lemma
-    (requires
-      interp (pts_to x v0 `star` pts_to x v1) m)
-    (ensures
-      composable pcm v0 v1 /\
-      interp (pts_to x (op pcm v0 v1)) m)
-  = let c = select_addr m x in
-    let Ref _ _ v = select_addr m x in
-    let aux (c0 c1: cell u#a)
-      : Lemma
-        (requires
-           c0 `disjoint_cells` c1 /\
-           interp_cell (pts_to x v0) c0 /\
-           interp_cell (pts_to x v1) c1 /\
-           c == join_cells c0 c1 )
-        (ensures
-           composable pcm v0 v1 /\
-           interp (pts_to x (op pcm v0 v1)) m)
-        [SMTPat (c0 `disjoint_cells` c1)]
-      = let Ref _ _ v0' = c0 in
-        let Ref _ _ v1' = c1 in
-        assert (exists frame. composable pcm v0 frame /\ op pcm frame v0 == v0');
-        assert (exists frame. composable pcm v1 frame /\ op pcm frame v1 == v1');
-        assert (composable pcm v0' v1');
-        assert (op pcm v0' v1' == v);
-        let aux (frame0 frame1:a)
-          : Lemma
-            (requires
-              composable pcm v0 frame0 /\
-              op pcm frame0 v0 == v0' /\
-              composable pcm v1 frame1 /\
-              op pcm frame1 v1 == v1')
-            (ensures (
-              composable pcm frame0 frame1 /\
-              composable pcm v0 v1 /\
-              (let frame = op pcm frame0 frame1 in
-               composable pcm frame (op pcm v0 v1) /\
-               op pcm frame (op pcm v0 v1) == v)))
-            [SMTPat(op pcm frame0 v0);
-             SMTPat(op pcm frame1 v1)]
-          =  assert (op pcm (op pcm frame0 v0) (op pcm frame1 v1) == v);
-             pcm.assoc (op pcm frame0 v0) frame1 v1;
-             assert (op pcm (op pcm (op pcm frame0 v0) frame1) v1 == v);
-             pcm.comm  (op pcm frame0 v0) frame1;
-             assert (op pcm (op pcm frame1 (op pcm frame0 v0)) v1 == v);
-             pcm.assoc_r frame1 (op pcm frame0 v0) v1;
-             assert (op pcm frame1 (op pcm (op pcm frame0 v0) v1) == v);
-             pcm.assoc_r frame0 v0 v1;
-             assert (op pcm frame1 (op pcm frame0 (op pcm v0 v1)) == v);
-             pcm.assoc frame1 frame0 (op pcm v0 v1);
-             pcm.comm frame1 frame0
-        in
-        ()
-    in
-    assert (exists c0 c1.
-              c0 `disjoint_cells` c1 /\
-              interp_cell (pts_to x v0) c0 /\
-              interp_cell (pts_to x v1) c1 /\
-              c == join_cells c0 c1)
+                      (m:mem u#a)
+  = H.pts_to_compatible x v0 v1 (heap_of_mem m)
 
 ////////////////////////////////////////////////////////////////////////////////
 // star
 ////////////////////////////////////////////////////////////////////////////////
 
-let intro_star (p q:slprop) (mp:hheap p) (mq:hheap q)
-  : Lemma
-    (requires
-      disjoint mp mq)
-    (ensures
-      interp (p `star` q) (join mp mq))
-  = ()
+let intro_star p q mp mq =
+  H.intro_star p q (heap_of_mem mp) (heap_of_mem mq)
 
+let star_commutative (p1 p2:slprop) =
+  H.star_commutative p1 p2
 
-(* Properties of star *)
+let star_associative (p1 p2 p3:slprop) =
+  H.star_associative p1 p2 p3
 
-let star_commutative (p1 p2:slprop) = ()
+let star_congruence (p1 p2 p3 p4:slprop) =
+  equiv_heap_iff_equiv_forall ();
+  H.star_congruence p1 p2 p3 p4
 
-let star_associative (p1 p2 p3:slprop)
-  = let ltor (m m1 m2 m3:heap)
-    : Lemma
-      (requires
-        disjoint m2 m3 /\
-        disjoint m1 (join m2 m3) /\
-        m == join m1 (join m2 m3) /\
-        interp p1 m1 /\
-        interp p2 m2 /\
-        interp p3 m3 /\
-        interp (p1 `star` (p2 `star` p3)) m)
-      (ensures
-        disjoint m1 m2 /\
-        disjoint (join m1 m2) m3 /\
-        m == join (join m1 m2) m3 /\
-        interp (p1 `star` p2) (join m1 m2) /\
-        interp ((p1 `star` p2) `star` p3) m)
-      [SMTPat()]
-    = disjoint_join m1 m2 m3;
-      join_associative m1 m2 m3;
-      intro_star p1 p2 m1 m2;
-      intro_star (p1 `star` p2) p3 (join m1 m2) m3
-   in
-   let rtol (m m1 m2 m3:heap)
-    : Lemma
-      (requires
-        disjoint m1 m2 /\
-        disjoint (join m1 m2) m3 /\
-        m == join (join m1 m2) m3 /\
-        interp p1 m1 /\
-        interp p2 m2 /\
-        interp p3 m3 /\
-        interp ((p1 `star` p2) `star` p3) m)
-      (ensures
-        disjoint m2 m3 /\
-        disjoint m1 (join m2 m3) /\
-        m == join m1 (join m2 m3) /\
-        interp (p2 `star` p3) (join m2 m3) /\
-        interp (p1 `star`(p2 `star` p3)) m)
-      [SMTPat()]
-    = join_associative2 m1 m2 m3;
-      intro_star p2 p3 m2 m3;
-      intro_star p1 (p2 `star` p3) m1 (join m2 m3)
-   in
-   ()
-
-let star_congruence (p1 p2 p3 p4:slprop) = ()
-
+let affine_star (p q:slprop) (m:mem) =
+  H.affine_star p q (heap_of_mem m)
 
 ////////////////////////////////////////////////////////////////////////////////
-// sel
+// Invariants on the lock store
 ////////////////////////////////////////////////////////////////////////////////
-let sel #a #pcm (r:ref a pcm) (m:hheap (ptr r))
-  : a
-  = let Ref _ _ v = select_addr m r in
-    v
 
-let sel_lemma (#a:_) (#pcm:_) (r:ref a pcm) (m:hheap (ptr r))
-  : Lemma (interp (pts_to r (sel r m)) m)
-  = let Ref _ _ v = select_addr m r in
-    assert (sel r m == v);
-    compatible_refl pcm v
+let lock_addr = nat
+module S = FStar.Set
+module L = FStar.List.Tot
+let rec lock_store_invariant (e:S.set lock_addr) (l:lock_store u#a) : slprop u#a =
+  let current_addr = L.length l - 1 in
+  match l with
+  | [] -> emp
+  | Invariant p :: tl ->
+    if current_addr `S.mem` e then
+      lock_store_invariant e tl
+    else
+      p `star` lock_store_invariant e tl
 
-let sel_action (#a:_) (#pcm:_) (r:ref a pcm) (v0:erased a)
-  : action (pts_to r v0) (v:a{compatible pcm v0 v}) (fun _ -> pts_to r v0)
-  = let f
-      : pre_action (pts_to r v0)
-                   (v:a{compatible pcm v0 v})
-                   (fun _ -> pts_to r v0)
-      = fun m0 -> (| sel r m0, m0 |)
-    in
-    f
+let heap_ctr_valid (ctr:nat) (h:H.heap u#a) : H.a_heap_prop u#a =
+  fun _ -> h `H.free_above_addr` ctr
 
+let locks_invariant (e:S.set lock_addr) (m:mem u#a) : slprop u#a =
+  H.h_refine (lock_store_invariant e m.locks)
+             (heap_ctr_valid m.ctr (heap_of_mem m))
 
-let upd' (#a:_) (#pcm:_) (r:ref a pcm) (v0:FStar.Ghost.erased a) (v1:a {frame_preserving pcm v0 v1})
-  : pre_action (pts_to r v0) unit (fun _ -> pts_to r v1)
-  = fun h ->
-    let cell = Ref a pcm v1  in
-    let h' = update_addr h r cell in
-    assert (h' `contains_addr` r);
-    compatible_refl pcm v1;
-    assert (interp_cell (pts_to r v1) cell);
-    assert (interp (pts_to r v1) h');
-    (| (), h' |)
+(***** Following lemmas are needed in Steel.Effect *****)
 
+let core_mem_interp (hp:slprop u#a) (m:mem u#a) = ()
 
-let definedness #a #pcm (v0:a) (v0_val:a) (v1:a) (vf:a)
-  : Lemma (requires
-             compatible pcm v0 v0_val /\
-             composable pcm v0_val vf /\
-             frame_preserving pcm v0 v1)
-          (ensures
-             composable pcm vf v1 /\
-             composable pcm v1 vf)
-  = assert (exists vf'. composable pcm vf' v0 /\ op pcm vf' v0 == v0_val);
-    let aux (vf':a {composable pcm vf' v0 /\ op pcm vf' v0 == v0_val})
-      : Lemma (composable pcm vf v1 /\
-               composable pcm v1 vf)
-              [SMTPat(op pcm vf' v0)]
-        = assert (composable pcm (op pcm vf' v0) vf);
-          pcm.comm vf' v0;
-          assert (composable pcm (op pcm v0 vf') vf);
-          pcm.assoc_r v0 vf' vf;
-          assert (composable pcm v0 (op pcm vf' vf));
-          pcm.comm vf vf';
-          assert (composable pcm v0 (op pcm vf vf'));
-          assert (composable pcm (op pcm vf vf') v1);
-          pcm.comm (op pcm vf vf') v1;
-          pcm.assoc v1 vf vf';
-          assert (composable pcm (op pcm v1 vf) vf')
-    in
-    ()
+let interp_depends_only_on (hp:slprop u#a) = H.interp_depends_only_on hp
 
-let composable_compatible #a pcm (x y z:a)
-  : Lemma (requires compatible pcm x y /\
-                    composable pcm y z)
-          (ensures composable pcm x z /\
-                   composable pcm z x)
-  = let aux (f:a{composable pcm f x /\ op pcm f x == y})
-      : Lemma (composable pcm x z /\
-               composable pcm z x)
-              [SMTPat (op pcm f x)]
-      = assert (composable pcm (op pcm f x) z);
-        pcm.assoc_r f x z;
-        assert (composable pcm f (op pcm x z));
-        pcm.comm x z
-    in
-    let s : squash (exists f. composable pcm f x /\ op pcm f x == y) = () in
-    ()
-
-#push-options "--z3rlimit_factor 2"
-let upd_lemma' (#a:_) #pcm (r:ref a pcm)
-               (v0:Ghost.erased a) (v1:a {frame_preserving pcm v0 v1})
-               (h:hheap (pts_to r v0)) (frame:slprop)
-  : Lemma
-    (requires
-      interp (pts_to r v0 `star` frame) h)
-    (ensures (
-      (let (| x, h1 |) = upd' r v0 v1 h in
-       interp (pts_to r v1 `star` frame) h1)))
-  = let aux (h0 hf:heap)
-     : Lemma
-       (requires
-         disjoint h0 hf /\
-         h == join h0 hf /\
-         interp (pts_to r v0) h0 /\
-         interp frame hf)
-       (ensures (
-         let (| _, h' |) = upd' r v0 v1 h in
-         let h0' = update_addr h0 r (Ref a pcm v1) in
-         disjoint h0' hf /\
-         interp (pts_to r v1) h0' /\
-         interp frame hf /\
-         h' == join h0' hf))
-       [SMTPat (disjoint h0 hf)]
-     = let (| _, h'|) = upd' r v0 v1 h in
-       let cell1 = (Ref a pcm v1) in
-       let h0' = update_addr h0 r cell1 in
-       assert (interp (pts_to r v1) h0');
-       assert (interp frame hf);
-       let aux (a:addr)
-         : Lemma (disjoint_addr h0' hf a )
-                 [SMTPat (disjoint_addr h0' hf a)]
-         = if a <> r then ()
-           else match h0 a, h0' a, hf a with
-                | Some (Ref a0 p0 v0_val),
-                  Some (Ref a0' p0' v0'),
-                  Some (Ref af pf vf) ->
-                  assert (a0' == af);
-                  assert (p0' == pf);
-                  assert (v0' == v1);
-                  assert (compatible pcm v0 v0_val);
-
-                  compatible_refl pcm vf;
-                  assert (interp_cell (pts_to r vf) (Some?.v (hf a)));
-                  assert (interp (pts_to r vf) hf);
-
-                  compatible_refl pcm v0_val;
-                  assert (interp_cell (pts_to r v0_val) (Some?.v (h0 a)));
-                  assert (interp (pts_to r v0_val) h0);
-                  assert (interp (pts_to r v0_val `star` pts_to r vf) h);
-                  pts_to_compatible r v0_val vf h;
-                  assert (composable pcm v0_val vf);
-
-                  assert (interp (pts_to r (op pcm v0_val vf)) h);
-                  pcm.comm v0_val vf;
-                  definedness #_ #pcm v0 v0_val v1 vf;
-                  assert (composable pcm v1 vf)
-                | _ -> ()
-       in
-       assert (disjoint h0' hf);
-       let aux (a:addr)
-         : Lemma (h' a == (join h0' hf) a)
-                 [SMTPat ()]
-         = if a <> r
-           then ()
-           else begin
-             assert (h' a == Some cell1);
-             assert (h0' a == Some cell1);
-             match h0 a, hf a with
-             | _, None -> ()
-             | Some (Ref a0 p0 v0_val),
-               Some (Ref af pf vf) ->
-               let c0 = Some?.v (h0 a) in
-               let cf = Some?.v (hf a) in
-               assert (a0 == af);
-               assert (p0 == pf);
-               assert (compatible pcm v0 v0_val);
-               assert (disjoint_cells c0 cf);
-               assert (composable pcm v0_val vf);
-               composable_compatible pcm v0 v0_val vf;
-               assert (composable pcm v0 vf);
-               assert (disjoint_cells cell1 cf);
-               assert (composable pcm v1 vf);
-               assert (composable pcm vf v0);
-               assert (op pcm vf v1 == v1);
-               pcm.comm vf v1
-           end
-       in
-       assert (mem_equiv h' (join h0' hf))
-   in
-   ()
-#pop-options
-
-let upd_action (#a:_) (#pcm:_) (r:ref a pcm) (v0:FStar.Ghost.erased a) (v1:a {frame_preserving pcm v0 v1})
-  : action (pts_to r v0) unit (fun _ -> pts_to r v1)
-  = let aux (h:hheap (pts_to r v0)) (frame:slprop)
+let h_exists_cong (#a:Type) (p q : a -> slprop)
     : Lemma
-      (requires
-        interp (pts_to r v0 `star` frame) h)
-      (ensures (
-        (let (| x, h1 |) = upd' r v0 v1 h in
-        interp (pts_to r v1 `star` frame) h1)))
-      [SMTPat ( interp (pts_to r v0 `star` frame) h)]
-    = upd_lemma' r v0 v1 h frame
+      (requires (forall x. p x `equiv` q x))
+      (ensures (h_exists p `equiv` h_exists q))
+    = equiv_heap_iff_equiv_forall ();
+      H.h_exists_cong p q
+
+////////////////////////////////////////////////////////////////////////////////
+// Lifting heap actions
+////////////////////////////////////////////////////////////////////////////////
+
+let linv (m:mem) = locks_invariant Set.empty m
+
+let hheap_of_hmem #fp (m:hmem_with_inv fp) : H.hheap (fp `star` linv m) =
+  heap_of_mem m
+
+let hmem_of_hheap (#fp0 #fp1:slprop) (m:hmem_with_inv fp0)
+                  (h:H.hheap (fp1 `star` linv m) {
+                    forall ctr. heap_of_mem m `H.free_above_addr` ctr <==>
+                           h `Heap.free_above_addr` ctr
+                  })
+    : hmem_with_inv fp1
+    = let m1 : mem = { m with heap = h } in
+      assert (interp (fp1 `star` linv m) m1);
+      star_commutative fp1 (linv m);
+      assert (interp (linv m `star` fp1) m1);
+      assert (linv m1 ==  H.h_refine (lock_store_invariant S.empty m1.locks)
+                                     (heap_ctr_valid m1.ctr (heap_of_mem m1)));
+      assert (linv m ==  H.h_refine (lock_store_invariant S.empty m1.locks)
+                                    (heap_ctr_valid m1.ctr (heap_of_mem m)));
+      assert (forall h. (heap_ctr_valid m1.ctr (heap_of_mem m)) h <==>
+                   (heap_ctr_valid m1.ctr (heap_of_mem m1)) h);
+      H.refine_equiv (lock_store_invariant S.empty m1.locks)
+                     (lock_store_invariant S.empty m1.locks)
+                     (heap_ctr_valid m1.ctr (heap_of_mem m))
+                     (heap_ctr_valid m1.ctr (heap_of_mem m1));
+      assert (linv m `equiv` linv m1);
+      let _ = equiv_extensional_on_star (linv m) (linv m1) fp1 in
+      assert ((linv m `star` fp1) `equiv` (linv m1 `star` fp1));
+      assert (interp (linv m1 `star` fp1) m1);
+      star_commutative (linv m1) fp1;
+      assert (interp (fp1 `star` linv m1) m1);
+      m1
+
+let ac_reasoning_for_m_frame_preserving _ _ _ _ = admit()
+
+let with_inv (m:mem) (fp:slprop) = interp (fp `star` locks_invariant Set.empty m) m
+
+#push-options "--warn_error -271"
+let as_hprop (frame:slprop) (mp:mprop frame)
+    : hp:H.hprop frame{forall m. mp (core_mem m) == hp (heap_of_mem m)}
+    = let f = fun h -> mp (mem_of_heap h) in
+      assert (forall m. mp (core_mem m) == f (heap_of_mem m));
+      let aux (m0:H.hheap frame) (m1:H.heap{H.disjoint m0 m1})
+        : Lemma
+          (ensures (mem_of_heap (H.join m0 m1) == join (mem_of_heap m0) (mem_of_heap m1)))
+          [SMTPat ()]
+        = ()
+      in
+      f
+
+let lift_heap_action (#fp:slprop) (#a:Type) (#fp':a -> slprop)
+                     ($f:H.action fp a fp')
+  : action fp a fp'
+  = let g : pre_action fp a fp' = fun m ->
+        let h0 = hheap_of_hmem m in
+        let (| x, h' |) = f h0 in
+        (| x, hmem_of_hheap m h' |)
     in
-    upd' r v0 v1
+    let aux (frame:slprop) (m0:hmem_with_inv (fp `star` frame))
+      : Lemma
+        (ensures
+          (ac_reasoning_for_m_frame_preserving fp frame (locks_invariant Set.empty m0) m0;
+           let (| x, m1 |) = g m0 in
+           interp ((fp' x `star` frame) `star` locks_invariant Set.empty m1) m1 /\
+           (forall (mp:mprop frame). mp (core_mem m0) == mp (core_mem m1))))
+        [SMTPat ()]
+      = ac_reasoning_for_m_frame_preserving fp frame (locks_invariant Set.empty m0) m0;
+        let (| x, m1 |) = g m0 in
+        let h0 = hheap_of_hmem m0 in
+        let (| x', h1 |) = f h0 in
+        H.action_framing f (linv m0) h0;
+        assert (x == x');
+        star_associative fp frame (linv m0);
+        H.action_framing f (frame `star` linv m0) h0;
+        assert (H.interp ((fp' x) `star` (frame `star` linv m0)) h1);
+        star_associative (fp' x) frame (linv m0);
+        assert (H.interp ((fp' x `star` frame) `star` linv m0) h1);
+        let h1' : H.hheap ((fp' x `star` frame) `star` linv m0) = h1 in
+        assert (m1 == hmem_of_hheap m0 h1');
+        assert (with_inv m1 (fp' x `star` frame));
+        assert (forall (hp:H.hprop frame). hp h0 == hp h1);
+        let aux_h (hp:H.hprop frame)
+          : Lemma (hp h0 == hp h1)
+          = ()
+        in
+        let aux (mp:mprop frame)
+          : Lemma
+            (ensures mp (core_mem m0) == mp (core_mem m1))
+            [SMTPat ()]
+          = assert (core_mem m1 == (core_mem ({m0 with heap = h1})));
+            assert (heap_of_mem m0 == h0);
+            let q = as_hprop frame mp in
+            assert (mp (core_mem m0) == q h0);
+            aux_h q
+        in
+        ()
+    in
+    assert (is_frame_preserving g);
+    g
+
+let sel_action r v0
+  = lift_heap_action (H.sel_action r v0)
+
+let upd_action r v0 v1
+  = lift_heap_action (H.upd_action r v0 v1)
